%Exercicio324
%exercicio 480
\begin{ex}
\begin{align}
&y=\ln{\frac{x^2+\sqrt{2}x+1}{x^2-\sqrt{2}x+1}}\nonumber\\
%resposta
&y'=\frac{x^2-\sqrt{2}x+1}{x^2+\sqrt{2}x+1}.\frac{(2x+\sqrt{2})(x^2-\sqrt{2}x+1)}{(x^2-\sqrt{2}x+1)^2}+\nonumber\\
&-\frac{(2x-\sqrt{2})(x^2+\sqrt{2}x+1)}{(x^2-\sqrt{2}x+1)^2}\nonumber\\
&y'=\frac{[2x(x^2+1)+\sqrt{2}(x^2+1)-2\sqrt{2}x^2-2x]}{[(x^2+1)+\sqrt{2}x]^2}+\nonumber\\
&y'=-\frac{[2x(x^2+1)-\sqrt{2}(x^2+1)+\sqrt{2}(x^2+1)+2\sqrt{2}x^2-2x]}{[(x^2+1)-\sqrt{2}x]^2}\nonumber\\
&y'=\frac{2\sqrt{2}(x^2+1)-4\sqrt{2}x^2}{(x^2+1)^2-2x^2}\nonumber\\
&y'=\frac{2\sqrt{2}(1-x^2)}{x^4+1}\nonumber
\end{align}
\end{ex}
