%Exercicio111
%exercicio 216
\begin{ex}
\begin{align}
&\lim_{b\rightarrow a} \frac{\sqrt{x^2-a+b}-\sqrt{x^2+a-b}}{a^2-b^2}=\nonumber\\
%resposta
&\text{multiplicando e dividindo pelo conjugado do numerador, temos:}\nonumber\\
&\lim_{b\rightarrow a} \frac{(\sqrt{x^2-a+b}-\sqrt{x^2+a-b})(\sqrt{x^2-a+b}+\sqrt{x^2+a-b})}{(a^2-b^2)(\sqrt{x^2-a+b}+\sqrt{x^2+a-b})}=\nonumber\\
&\lim_{b\rightarrow a} \frac{(x^2-a+b)-(x^2+a-b)}{(a+b)(a-b)(\sqrt{x^2-a+b}+\sqrt{x^2+a-b})}=\nonumber\\
&\lim_{b\rightarrow a} \frac{-2(a-b)}{(a+b)(a-b)(\sqrt{x^2-a+b}+\sqrt{x^2+a-b})}=\nonumber\\
&\frac{-2}{46\sqrt{x^2}}=\frac{-2}{4bx}=\frac{-1}{2bx}\nonumber
\end{align}
\end{ex}
