%Exercicio93
%exercicio 186
\begin{ex}
\begin{align}
&\lim_{x\rightarrow \infty} \frac{(2x-1)^2}{x(x+3)}=\nonumber\\
%resposta
&\lim_{x\rightarrow \infty} \frac{4x^2-4x+1}{x^2+3x}=\nonumber\\
&\text{dividindo-se o numerador e o denominador por}\quad x^2,\quad\text{temos:}\nonumber\\
&\lim_{x\rightarrow \infty} \frac{\frac{4x^2}{x^2}-\frac{4x}{x^2}+\frac{1}{x^2}}{\frac{x^2}{x^2}+\frac{3x}{x^2}}=\lim_{x\rightarrow \infty} \frac{4-\frac{4}{x}+\frac{1}{x^2}}{1+\frac{3}{x}}=\frac{4}{1}=4\nonumber
\end{align}
\end{ex}
