%Exercicio399
%exercicio 558
\begin{ex}
\begin{align}
&\lim_{x\rightarrow 0} \left[\frac{1}{2x}-\frac{1}{x(e^{ax}+1)}\right]\nonumber\\
%resposta
&\lim_{x\rightarrow 0} \left[\frac{1}{2x}-\frac{1}{x(e^{ax}+1)}\right]= [\infty-\infty]\nonumber\\
&\lim_{x\rightarrow 0} \frac{e^{ax}+1-2}{2x(e^{ax}+1)}=\left[\frac{0}{0}\right]\nonumber\\
&\lim_{x\rightarrow 0} \frac{e^{ax}-1}{2x(e^{ax}+1)}=\left[\frac{0}{0}\right]\nonumber\\
&\lim_{x\rightarrow 0} \frac{ae^{ax}}{2(e^{ax}+1)+2axe^{ax}}=\frac{3}{4}=\frac{a}{4}\nonumber
\end{align}
\end{ex}