%Exercicio326
%exercicio 482
\begin{ex}
\begin{align}
&y=\ln{\sqrt[3]{\frac{\cos{x}+\sen{x}}{\cos{x}-\sen{x}}}}\nonumber\\
%resposta
&y=\frac{1}{3}\ln{(\cos{x}+\sen{x})}-\frac{1}{3}\ln{(\cos{x}-\sen{x})}\nonumber\\
&y'=\frac{1}{3}\frac{1}{(\cos{x}+\sen{x})}(\cos{x}-\sen{x})+\frac{1}{3}\frac{1}{(\cos{x}+\sen{x})}(\sen{x}+\cos{x})\nonumber\\
&y'=\frac{1}{3}\frac{(\cos{x}-\sen{x})}{(\cos{x}+\sen{x})}+\frac{1}{3}\frac{(\sen{x}+\cos{x})}{(\cos{x}-\sen{x})}\nonumber\\
&y'=\frac{1}{3}\frac{(\cos{x}-\sen{x})^2+(\cos{x}+\sen{x})^2}{\cos^2{x}-\sen^2{x}}\nonumber\\
&y'=\frac{1}{3}\frac{(2\cos^2{x}+2\sen^2{x})}{\cos{2x}}=\frac{2}{3\cos{2x}}\nonumber
\end{align}
\end{ex}