%Exercicio17
%exercicio166
\begin{ex}
\begin{align}
&\lim_{x\rightarrow 1} \left[\frac{1}{x-1}-\frac{3}{1-x^3}\right]\nonumber\\
%resposta
&\lim_{x\rightarrow 1} \left[\frac{1+x+x^2-3}{(1-x)(1+x+x^2)}\right] = \lim_{x\rightarrow 1} \frac{(x^2+1)(x-1)(x+1)}{(x-1)(x-1)}\nonumber\\
&\text{e fatorando-se}\quad x^2+x-2=(x-1)(x+1),\quad \text{temos:}\nonumber\\
&\lim_{x\rightarrow 1} \frac{(x-1)(x+2)}{(1-x)(1+x+x^2)}=\lim_{x\rightarrow 1} -\frac{x+2}{1+x+x^2}=-\frac{3}{3}=-1\nonumber
\end{align}
\end{ex}