%Exercicio246
%exercicio 402
\begin{ex}
\begin{align}
&y=2.\frac{\sqrt{a^2+e^x}-a}{\sqrt{e^x}}+\sen{x}\nonumber\\
%resposta
&y'=2.\frac{\sqrt{e^x}}{\sqrt{a^2+e^x}-a}.\frac{\frac{\frac{1}{2}}{\sqrt{a^2+e^x}}.e^x.\sqrt{e^x}-\frac{e^x}{2\sqrt{e^x}}.(\sqrt{a^2+e^x}-a)}{e^x}+\cos^{x}\nonumber\\
&y'=2.\frac{\sqrt{e^x}}{\sqrt{a^2+e^x}-a}.\frac{1}{2}\left(\frac{\sqrt{e^x}}{\sqrt{a^2+e^x}}-\frac{\sqrt{a^2+e^x}-a}{\sqrt{e^x}}\right)\nonumber\\
&y'=\frac{2}{2}.\frac{\sqrt{e^x}}{\sqrt{a^2+e^x}-a}.\frac{e^x-a^2-e^x+a\sqrt{a^2+e^x}}{\sqrt{e^x(a^2+e^x)}}+\cos{x}\nonumber\\
&y'=\frac{a(\sqrt{a^2+e^x}-a)}{(\sqrt{a^2+e^x}-a)\sqrt{a^2+e^x}}+\cos{x}=\frac{a}{2\sqrt{a^2+e^x}}+\cos{x}\nonumber
\end{align}
\end{ex}