%Exercicio411
%exercicio 572
\begin{ex}
\begin{align}
&\lim_{x\rightarrow 0} \left(\frac{1}{x}-\frac{1}{e^{x}-1}\right)\nonumber\\
%resposta
&\lim_{x\rightarrow 0} \left(\frac{1}{x}-\frac{1}{e^{x}-1}\right)=[\infty-\infty]\nonumber\\
&\lim_{x\rightarrow 0} \frac{e^{x}-1-1}{x(e^{x}-1)}=\left[\frac{0}{0}\right]\nonumber\\
&\lim_{x\rightarrow 0} \frac{e^{x}-1}{(e^{x}-1)+x.e^{x}}=\left[\frac{0}{0}\right]\nonumber\\
&\lim_{x\rightarrow 0} \frac{e^{x}}{xe^{x}+2e^{x}}=\frac{1}{2}\nonumber
\end{align}
\end{ex}