%Exercicio104
%exercicio 207
\begin{ex}
\begin{align}
&\lim_{x\rightarrow 1} \frac{\sqrt{x+3}-\sqrt{3x+1}}{x-1}=\nonumber\\
%resposta
&\lim_{x\rightarrow 1} \frac{(\sqrt{x+3}-\sqrt{3x+1})(\sqrt{x+3}+\sqrt{3x+1})}{(\sqrt{x+3}+\sqrt{3x+1})(x-1)}=\nonumber\\
&\lim_{x\rightarrow 1} \frac{(x+3-3x-1)}{(x-1)(\sqrt{x+3}+\sqrt{3x+1})}=\nonumber\\
&\lim_{x\rightarrow 1} \frac{(-2x+2)}{(x-1)}(\sqrt{x+3}+\sqrt{3x+1})=\nonumber\\
&\lim_{x\rightarrow 1} \frac{-2(x-1)}{(x-1)(\sqrt{x+3}+\sqrt{3x+1})}=\nonumber\\
&\lim_{x\rightarrow 1} \frac{-2}{\sqrt{x+3}+\sqrt{3x+1}}=\frac{-2}{\sqrt{1+3}+\sqrt{3+1}}=\nonumber\\
&\frac{-2}{\sqrt{4}+\sqrt{4}}=\sqrt{-2}{4}=-\frac{1}{2}\nonumber
\end{align}
\end{ex}
