%Exercicio242
%exercicio 398
\begin{ex}
\begin{align}
&y=\frac{x^3}{\sqrt{(1=x^2)^3}}\nonumber\\
%resposta
&y'=\frac{3x^2\sqrt{(1+x^2)^3}-\frac{1}{2}.\frac{x^3}{\sqrt{(1+x^2)^3}}.3(1+x^2).2x}{(1+x^2)^3}\nonumber\\
&y'=\frac{3x^2\sqrt{(1+x^2)^3}-\frac{3x^4(1+x^2)^2}{\sqrt{(1+x^2)^3}}}{(1+x^2)^3}\nonumber\\
&y'=\frac{3x^2(1+x^2)^3-3x^4(1+x^2)^2}{(1+x^2)^3\sqrt{(1+x^2)^3}}=\frac{3x^2(1+x^2)^2(1+x^2-x^2)}{(1+x^2)^3\sqrt{(1+x^2)^3}}\nonumber\\
&y'=\frac{3x^2}{(1+x^2)\sqrt{(1+x^2)^3}}=\frac{3x^2}{\sqrt(1+x^2)^5}=3x^2(1+x^2)-\frac{5}{2}\nonumber
\end{align}
\end{ex}