%Exercicio193
%exercicio 339
\begin{ex}
\begin{align}
&y=\frac{x+1}{x^2-1}\nonumber\\
%resposta
&y'=\frac{(x^2-1)(x+1)'(x^2-1)'(x+1)}{(x^2-1)^2}\nonumber\\
&y'=\frac{(x^2-1)(1)-(2x)(x+1)}{(x^2-1)^2}\nonumber\\
&y'=\frac{x^2-1-2x^2-2x}{(x^2-1)^2}=\frac{-x^2-2x-1}{(x^2-1)^2}\nonumber\\
&y'=\frac{-(x+1)^2}{(x^2-1)^2}=\frac{-(x+1)^2}{(x-1)^2(x+1)^2}=\frac{-1}{(x-1)^2}\nonumber\\
<<<<<<< HEAD
&\text{ou ent�o, se}\quad y=\frac{x+1}{x^2-1}\Rightarrow y=\frac{x+1}{(x-1)(x+1)}=\frac{1}{x-1}\nonumber\\
=======
&\text{ou ent�o, se}\quad y=\frac{x+1}{x^2-1}\Rightarrow y=\frac{x+1}{(x-1)(x+1)}=\frac{1}{x-1}\nonumber\\
>>>>>>> 2edfa61f09aa52eb0e5cbaaba256a294c2d4af48
&\text{logo se}\quad y=\frac{1}{x-1} \Rightarrow y'=\frac{1}{(x-1)^2}\nonumber
\end{align}
\end{ex}