%Exercicio161
%exercicio 298
\begin{ex}
\begin{align}
&y=\sqrt{x}\nonumber\\
%resposta
&y'=\lim_{h\rightarrow 0} \frac{\sqrt{x+h}-\sqrt{x}}{h}=\nonumber\\
&\text{multiplicando-se o numerador e o denominador por}\quad\sqrt{x+h}+\sqrt{x},\quad\text{temos:}\nonumber\\
&y'=\lim_{h\rightarrow 0} \frac{(\sqrt{x+h}-\sqrt{x})(\sqrt{x+h}+\sqrt{x})}{h(\sqrt{x+h}+\sqrt{x})}=\nonumber\\
&y'=\lim_{h\rightarrow 0} \frac{x+h-x}{h(\sqrt{x+h+x})}=\nonumber\\
&y'=\lim_{h\rightarrow 0} \frac{h}{h(\sqrt{x+h}+\sqrt{x})}=\lim_{h\rightarrow 0} \frac{1}{\sqrt{x+h}+\sqrt{x}}=\frac{1}{2\sqrt{x}}\nonumber
\end{align}
\end{ex}