%Exercicio196
%exercicio 342
\begin{ex}
\begin{align}
&y=\sqrt{\frac{x-1}{x+1}}\nonumber\\
%resposta
&y=\frac{\sqrt{x-1}}{\sqrt{x+1}}\nonumber\\
&y'=\frac{(\sqrt{x+1})(\sqrt{x-1})'-(\sqrt{x+1})'(\sqrt{x-1})}{(\sqrt{x+1})^2}\nonumber\\
&y'=\frac{\sqrt{x+1}.\frac{1}{2\sqrt{x-1}}-\sqrt{x-1}.\frac{1}{2\sqrt{x+1}}}{x+1}\nonumber\\
&y'=\frac{\frac{\sqrt{x+1}\sqrt{x+1}-\sqrt{x-1}\sqrt{x-1}}{2\sqrt{x-1}\sqrt{x+1}}}{(x+1)}=\frac{\frac{x+1-x+1}{2\sqrt{x-1}{\sqrt{x+1}}}}{x+1}\nonumber\\
&y'=\frac{2}{2\sqrt{x+1}{\sqrt{x-1}(x+1)}}=\frac{1}{(x-1)^\frac{1}{2}(x+1)^\frac{1}{2}(x+1)}\nonumber\\
&y'=\frac{1}{(x-1)^\frac{1}{2}(x+1)^\frac{3}{2}}\nonumber
\end{align}
\end{ex}