%Exercicio114
%exercicio 220
\begin{ex}
\begin{align}
&\lim_{x\rightarrow \infty} (\sqrt[3]{x+1}-\sqrt[3]{x})=\nonumber\\
%resposta
&\text{sendo}\quad a^3-b^3=(a-b)(a^2+ab+b^2)\quad\text{temos que:}\nonumber\\
&[(x+1)-(x)]=(\sqrt[3]{x+1}-\sqrt[3]{x})(\sqrt[3]{(x+1)^2}+\sqrt[3]{x(x+1)}+\sqrt[3]{x^2}\nonumber\\
&\text{chamando de}\quad A=\sqrt[3]{(x+1)^2}+\sqrt[3]{x(x+1)}+\sqrt[3]{x^2}\nonumber\\
&\text{e multiplicando-se o numerador e denominador por A, temos:}\nonumber\\
&\lim_{x\rightarrow \infty} \frac{(\sqrt[3]{x+1}-\sqrt[3]{x}).A}{A}=\nonumber\\
&\lim_{x\rightarrow \infty} \frac{(\sqrt[3]{x+1}-\sqrt[3]{x})(\sqrt{(x+1)^2}+\sqrt[3]{x(x+1)}+\sqrt[3]{x^2})}{(\sqrt[3]{(x+1)^2}+\sqrt[3]{x(x+1)}+\sqrt[3]{x^2})}=\nonumber\\
&\lim_{x\rightarrow \infty} \frac{[(x+1)-(x)]}{\sqrt[3]{(x+1)^2}+\sqrt[3]{x(x+1)}+\sqrt[3]{x^2}}=0\nonumber
\end{align}
\end{ex}