%Exercicio275
%exercicio 431
\begin{ex}
\begin{align}
&y=\arctg{\sqrt{x^2+2x}}-\frac{\log{(x+1)}}{x^2+2x}\nonumber\\
%resposta
&y'=\frac{1}{1+x^2+2x}.\frac{1}{2}.\frac{1}{\sqrt{x^2+2x}}.(2x+2)-\frac{1\sqrt{x^2+2x}-\frac{\log{(x+1)(2x+2)}}{2\sqrt{x^2+2x}}}{(x+1)(x^2+2x)}\nonumber\\
&y'=\frac{x+1}{(x+1)^2\sqrt{x+2+2x}}-\frac{1}{(x+1)\sqrt{x^2+2x}}+\frac{\log{(x+1)(x+1)}}{(x^2+2x)(\sqrt{x^2+2x})}\nonumber\\
&y'=\frac{(x+1)\log(x+1)}{(x^2+2x)(\sqrt{x^2+2x})}=\frac{(x+1)\log{(x+1)}}{(x^2+2x)^\frac{3}{2}}\nonumber
\end{align}
\end{ex}