%Exercicio191
%exercicio 337
\begin{ex}
\begin{align}
&y=\frac{x+2}{x^2-4}\nonumber\\
%resposta
&y'=\frac{(x^2-4)(x+2)'-(x^2-4)'(x+2)}{(x^2-4)^2}\nonumber\\
&y'=\frac{(x^2-4)(1)-(2x)(x+2)}{(x^2-4)^2}=\frac{x^2-4-2x^2-4x}{(x^2-4)^2}\nonumber\\
&y'=\frac{-x^2-4x-4}{(x^2-4)^2}=\frac{-(x^2+4x+4)}{[(x-2)(x+2)]^2}\nonumber\\
&y'=\frac{(x+2)(x+2)}{(x-2)(x-2)(x+2)(x+2)}=\frac{1}{(x-2)^2}\nonumber\\
&\text{ou se}\quad y=\frac{x+2}{x^2-4} \Rightarrow y=\frac{x+2}{(x-2)(x+2)}=\frac{1}{x-2}\nonumber\\
&\text{logo}\quad y'=-\frac{1}{(x-2)^2}\nonumber
\end{align}
\end{ex}