%Exercicio109
%exercicio 214
\begin{ex}
\begin{align}
&\lim_{a\rightarrow b} \frac{\sqrt{x^2-a}-\sqrt{x^2-b}}{a-b}=\nonumber\\
%resposta
&\text{multiplicando e dividindo pelo conjugado do numerador, temos:}\nonumber\\
&\lim_{a\rightarrow b} \frac{(\sqrt{x^2-a}-\sqrt{x^2-b})(\sqrt{x^2-a}+\sqrt{x^2-b})}{(a-b)(\sqrt{x^2-a}+\sqrt{x^2-b})}=\nonumber\\
&\lim_{a\rightarrow b} \frac{(x^2-a)-(x^2-b)}{(a-b)(\sqrt{x^2-a}+\sqrt{x^2-b})}=\nonumber\\
&\lim_{a\rightarrow b} \frac{-(a-b)}{(a-b)(\sqrt{x^2-a}+\sqrt{x^2-b})}=\frac{-1}{2\sqrt{x^2-b}}\nonumber
\end{align}
\end{ex}
