%Exercicio418
%exercicio 579
\begin{ex}
\begin{align}
&\lim_{x\rightarrow \frac{\pi}{2}} \left(2-\frac{2x}{\pi}\right)^{\tg{x}}\nonumber\\
%resposta
&\lim_{x\rightarrow \frac{\pi}{2}} \left(2-\frac{2x}{\pi}\right)^{\tg{x}}=[1^\infty]\nonumber\\
&z=\left(2-\frac{2x}{\pi}\right)^{\tg{x}} \Rightarrow \ln{z}=\tg{x}\ln{\left(2-\frac{2x}{\pi}\right)}\nonumber\\
&\lim_{x\rightarrow \frac{\pi}{2}} \ln{z}=\lim_{x\rightarrow \frac{\pi}{2}} \tg{x}\ln{\left(2-\frac{2x}{\pi}\right)}\nonumber\\
&\lim_{x\rightarrow \frac{\pi}{2}} \frac{\ln{\left(2-\frac{2x}{\pi}\right)}}{\cotg{x}}=\left[\frac{0}{0}\right]\nonumber\\
&\lim_{x\rightarrow \frac{\pi}{2}} \frac{\frac{1}{2-\frac{2x}{\pi}}.\left(\frac{2}{\pi}\right)}{-\frac{1}{\sen^2{x}}}=\lim_{x\rightarrow \frac{\pi}{2}} \frac{\frac{1}{\pi-x}}{\frac{1}{\sen^2{x}}}=\frac{2}{\pi}\nonumber\\
&\ln{z}=\frac{2}{\pi} \Rightarrow z=e^{\frac{2}{\pi}} \therefore \lim_{x\rightarrow \frac{\pi}{2}} \left(2-\frac{2x}{\pi}\right)^{\tg{x}}=e^{\frac{2}{\pi}}\nonumber
\end{align}
\end{ex}