%Exercicio110
%exercicio 215
\begin{ex}
\begin{align}
&\lim_{x\rightarrow \infty} (\sqrt{x^2+3x-1}-\sqrt{x^2-2x+3})=\nonumber\\
%resposta
&\text{multiplicando-se e dividindo-se pelo conjugado da expressão, temos:}\nonumber\\
&\lim_{x\rightarrow \infty} \frac{(\sqrt{x^2+3x-1}-\sqrt{x^2-2x+3})(\sqrt{x^2+3x-1}+\sqrt{x^2-2x+3})}{\sqrt{x^2+3x-1}+\sqrt{x^2-2x+3}}=\nonumber\\
&\lim_{x\rightarrow \infty} \frac{5}{\sqrt{1+\frac{3}{x}-\frac{1}{x^2}}+\sqrt{1-\sqrt{2}{x}+\frac{1}{x^2}}}=\frac{5}{2}\nonumber
\end{align}
\end{ex}