%Exercicio23
%exercicio 211
\begin{ex}
\begin{align}
&\lim_{x\rightarrow 1} \left(\frac{\sqrt{x}-1+\sqrt{x-1}}{\sqrt{x^2-1}}\right)=\nonumber\\
%resposta
&\lim_{x\rightarrow 1} \left(\frac{\sqrt{x}-1}{\sqrt{x^2-1}}+\frac{\sqrt{x-1}}{\sqrt{x^2-1}}\right)=\nonumber\\
&\lim_{x\rightarrow 1} \frac{(\sqrt{x}-1)(\sqrt{x^2-1})}{(\sqrt{x^2-1})(\sqrt{x^2-1})}=\frac{(\sqrt{x-1})(\sqrt{x^2-1})}{(\sqrt{x^2-1})(\sqrt{x^2-1})}=\nonumber\\
&\lim_{x\rightarrow 1} \frac{(\sqrt{x-1})(\sqrt{x^2-1})}{(x+1)(x-1)}+\frac{\sqrt{x-1}\sqrt{x+1}\sqrt{x-1}}{(x+1)(x-1)}=\nonumber\\
&\lim_{x\rightarrow 1} \left[\frac{\sqrt{x-1}\sqrt{x^2-1}}{(x+1)(x-1)}+\frac{\sqrt{x+1}}{x+1}\right]=\nonumber\\
&\lim_{x\rightarrow 1} \left[\frac{\sqrt{x^3-1}\sqrt{x-1}}{(x+1)(x-1)(\sqrt{x+1})}+\frac{\sqrt{x+1}}{x+1}\right]=
\frac{0}{2.2}+\frac{\sqrt{2}}{2}=\frac{\sqrt{2}}{2}\nonumber
\end{align}
\end{ex}