%Exercicio136
%exercicio 276
\begin{ex}
\begin{align}
&\lim_{x\rightarrow \infty} \left[\frac{1+3+5+\dots+(2x-1)}{x-1}-\frac{2x+1}{2}\right]=\nonumber\\
%resposta
&\text{sendo}\quad 1+3+5+\dots+(2x-1)=x^2,\quad\text{temos:}\nonumber\\
&\lim_{x\rightarrow \infty} \left[\frac{x^2}{x+1}-\frac{2x+1}{2}\right]=\lim_{x\rightarrow \infty} \frac{2x^2-(2x+1)(x+1)}{2(x+1)}=\nonumber\\
&\lim_{x\rightarrow \infty} \frac{2x^2-2x^2-2x-x-1}{2x+2}=\lim_{x\rightarrow \infty} \frac{-3x-1}{2x+2}=1,\nonumber\\
&\text{dividindo o numerador e o denominador por x temos}\nonumber\\
&\lim_{x\rightarrow \infty} \frac{-3-\frac{1}{x}}{2+\frac{2}{x}}=\frac{-3-0}{2+0}=\frac{3}{2}\nonumber
\end{align}
\end{ex}