%Exercicio343
%exercicio 499
\begin{ex}
\begin{align}
&y=\arccotg{x}\nonumber\\
&\text{Se}\quad y=\arccotg{x} \Rightarrow x= \cotg{y}\nonumber\\
&\text{derivando ambos os membros da equação, temos:}\nonumber\\
&-\frac{1}{\sen^2{y}}.y'=1 \Rightarrow y'=-\sen^2{y}\nonumber\\
&\text{podemos deduzir que:}\quad \sen{y}=\frac{1}{\sqrt{1+\cotg^2{y}}}\nonumber\\
&\text{como}\quad \cotg{y}=x, \quad \text{temos:}\quad \sen{y}=\frac{1}{\sqrt{1+x^2}}\nonumber\\
&\text{como} \quad y'=-\sen^2{y} \Rightarrow -\left(\frac{1}{\sqrt{1+x^2}}\right)^2\nonumber\\
&y'=\frac{-1}{1+x^2}\nonumber
\end{align}
\end{ex}
