%Exercicio382
%exercicio540
\begin{ex}
\begin{align}
&\lim_{x\rightarrow 0} \frac{e^{x}+e^{-x}-x^2-2}{\sen^2{x}-x^2}\nonumber\\
%resposta
&\lim_{x\rightarrow 0} \frac{e^{x}+e^{-x}-x^2-2}{\sen^2{x}-x^2}= \left[\frac{0}{0}\right]\nonumber\\
&\lim_{x\rightarrow 0} \frac{e^{x}-e^{-x}-2x}{2\sen{x}\cos{x}-2x}=\left[\frac{0}{0}\right]\nonumber\\
&\lim_{x\rightarrow 0} \frac{e^{x}+e^{_x}-2}{2\cos{2x}-2}=\left[\frac{0}{0}\right]\nonumber\\
&\lim_{x\rightarrow 0} \frac{e^{x}-e^{-x}}{-4\sen{2x}}=\left[\frac{0}{0}\right]\nonumber\\
&\lim_{x\rightarrow 0} \frac{e^{x}+e^{-x}}{-8\cos{2x}}=\frac{2}{-8}=-\frac{1}{4}\nonumber
\end{align}
\end{ex}