%Exercicio19
%exercicio213
\begin{ex}
\begin{align}
&\lim_{x\rightarrow \infty} \left(\sqrt{\frac{4x^3+3x^2}{4x-3}}-x\right)=\nonumber\\
%resposta
&text{multiplicando e dividindo pelo conjugado da expressão, temos:}\nonumber\\
&\lim_{x\rightarrow \infty} \frac{\frac{4x^3+3x^2}{4x-3}-x^2}{\sqrt{\frac{4x^3+3x^2}{4x-3}}+x}=\lim_{x\rightarrow \infty} \frac{\frac{6x^2}{4x-3}}{\sqrt{\frac{4x^3+3x^2}{4x-3}}+x}=\nonumber\\
&\lim_{x\rightarrow \infty} \frac{6x^2}{(4x-3)(\sqrt{\frac{4x^3+3x^2}{4x-3}}+x}=\nonumber\\
&\lim_{x\rightarrow \infty} \frac{6x^2}{\sqrt{(4x^3+3x^2)(4x-3)}+x(4x-3)}=\nonumber\\
&\text{dividindo-se o numerador e o denominador por} \quad x^2,\quad \text{temos:}\nonumber\\
&\lim_{x\rightarrow \infty} \frac{6}{\sqrt{(4+\frac{3}{x})(4-\frac{3}{x})}+4-\frac{3}{x}}=\frac{6}{4+4}=\frac{3}{4}\nonumber
\end{align}
\end{ex}