%Exercicio182
%exercicio 328
\begin{ex}
\begin{align}
&y=\frac{x^2-1}{x+1}\nonumber\\
%resposta
&y'=\frac{(x+1)(x^2-1)'-(x^2-1)(x+1)'}{(x+1)^2}\nonumber\\
&y'=\frac{(x+1)(2x)-(1)(x^2-1)}{(x+1)^2}\nonumber\\
&y'=\frac{2x^2+2x-x^2+1}{(x+1)^2}=\frac{x^2+2x+1}{(x+1)^2}=\frac{(x+1)^2}{(x+1)^2}=1\nonumber\\
<<<<<<< HEAD
&\text{ou então: se}\quad y=\frac{x^2-1}{x-1} \Rightarrow y=\frac{(x+1)(x-1)}{x-1}=x+1\nonumber\\
=======
&\text{ou entï¿½o: se}\quad y=\frac{x^2-1}{x-1} \Rightarrow y=\frac{(x+1)(x-1)}{x-1}=x+1\nonumber\\
>>>>>>> 2edfa61f09aa52eb0e5cbaaba256a294c2d4af48
&\text{logo se}\quad y=x+1 \Rightarrow y'=1\nonumber
\end{align}
\end{ex}
