%Exercicio122
%exercicio 259
\begin{ex}
\begin{align}
&\lim_{x\rightarrow \infty} \left(\frac{x+3}{x-1}\right)^{x+3}=\nonumber\\
%resposta
&\lim_{x\rightarrow \infty} \left(\frac{x-1+4}{x-1}\right)^{x+3}=\lim_{x\rightarrow \infty} \left(1+\frac{4}{x-1}\right)^{x+3}=\nonumber\\
&\lim_{x\rightarrow \infty} \left(1+\frac{4}{x-1}\right)^{(x-1)+4}=\nonumber\\
&\text { fazendo-se }\quad x-1=y,\quad \text { temos: } \quad \lim_{y\rightarrow \infty} \left(1+\frac{4}{y}\right)^{y+4}=\nonumber\\
&\lim_{y\rightarrow \infty} \left(1+\frac{4}{y}\right)^y.\lim_{y\rightarrow \infty} \left(1+\frac{4}{y}\right)^4 = e^4.1^4 = e^4\nonumber
\end{align}
\end{ex}