%Exercicio414
%exercicio 575
\begin{ex}
\begin{align}
&\lim_{x\rightarrow 0} \left(\frac{1}{x^2}-\cotg^2{x}\right)\nonumber\\
%resposta
&\lim_{x\rightarrow 0} \left(\frac{1}{x^2}-\cotg{x}\right)=[\infty-\infty]\nonumber\\
&\lim_{x\rightarrow 0} \left(\frac{1}{x^2}-\frac{\cos^2{x}}{\sen^2{x}}\right)=\lim_{x\rightarrow 0} \left(\frac{\sen^2{x}-x^2\cos^2{x}}{x^3\sen^2{x}}\right)=\left[\frac{0}{0}\right]\nonumber\\
&\lim_{x\rightarrow 0} \frac{\sen{2x}-2x\cos^2{x}+x^2\sen{2x}}{2x\sen^2{x}+x^2\sen{2x}}=\left[\frac{0}{0}\right]\nonumber\\
&\lim_{x\rightarrow 0} \frac{2\cos{2x}-2\cos^2{x}+2x\sen{2x}+2x^2\cos{2x}+2x\sen{2x}}{2\sen^2{x}+2x\sen{2x}+2x\sen{2x}+2x^2\cos{2x}}=\left[\frac{0}{0}\right]\nonumber\\
&\lim_{x\rightarrow 0} \frac{12x\cos{2x}-4x^2\sen{2x}+2\sen{2x}}{12x\cos{2x}+6\sen{2x}-4x^2\sen{2x}}=\left[\frac{0}{0}\right]\nonumber\\
&\lim_{x\rightarrow 0} \frac{-32x\sen{2x}+16\cos{2x}-8x^2\cos{2x}}{-32x\sen{2x}+24\cos{2x}-8x^2\cos{2x}}=\frac{16}{24}=\frac{2}{3}\nonumber
\end{align}
\end{ex}
