%Exercicio113
%exercicio 219
\begin{ex}
\begin{align}
&\lim_{x\rightarrow 1} \frac{\sqrt[3]{2x+6}-2}{x-1}=\nonumber\\
%resposta
&\lim_{x\rightarrow 1} \frac{\sqrt[3]{2x+6}-\sqrt[3]{8}}{x-1}=\nonumber\\
&\text{como}\quad a^3-b^3=(a-b)(a^2+ab+b^2),\quad\text{temos:}\nonumber\\
<<<<<<< HEAD
&(2x+6)-8=(\sqrt[3]{2x+6}-\sqrt[3]{8})(\sqrt[3]{(2x+6)^2}+\sqrt[3]{16x+48}+\sqrt[3]{8^2}),\quad\text{ent�o:}\nonumber\\
&\sqrt[3]{2x+6}-\sqrt{8}=\frac{(2x+6)-8}{\sqrt[3]{2x+6-2}+\sqrt[3]{16x+48}+\sqrt[3]{8^2}}=\nonumber\\
&\text{substituindo-se na express�o, temos:}\nonumber\\
=======
&(2x+6)-8=(\sqrt[3]{2x+6}-\sqrt[3]{8})(\sqrt[3]{(2x+6)^2}+\sqrt[3]{16x+48}+\sqrt[3]{8^2}),\quad\text{ent�o:}\nonumber\\
&\sqrt[3]{2x+6}-\sqrt{8}=\frac{(2x+6)-8}{\sqrt[3]{2x+6-2}+\sqrt[3]{16x+48}+\sqrt[3]{8^2}}=\nonumber\\
&\text{substituindo-se na express�o, temos:}\nonumber\\
>>>>>>> 2edfa61f09aa52eb0e5cbaaba256a294c2d4af48
&\lim_{x\rightarrow 1} \frac{\frac{(2x+6)-8}{\sqrt[3]{(2x+6)^2}+\sqrt[3]{16x+48}+\sqrt[3]{8^2}}}{(x-1)}=\nonumber\\
&\lim_{x\rightarrow 1} \frac{\frac{2(x-1)}{\sqrt[3]{(2x+6)^2}+\sqrt[3]{16x+48}+\sqrt[3]{8^2}}}{(x-1)}=\frac{2}{12}=\frac{1}{6}\nonumber
\end{align}
\end{ex}