%Exercicio192
%exercicio 38
\begin{ex}
\begin{align}
&y=\frac{a+\sqrt{x}}{a-\sqrt{x}}\nonumber\\
%resposta
&y'=\frac{(a-\sqrt{x})(a+\sqrt{x})'-(a-\sqrt{x})'(a+\sqrt{x})}{(a-\sqrt{x})^2}\nonumber\\
&y'=\frac{(a-\sqrt{x}).\frac{1}{2\sqrt{x}}-\left(\frac{-1}{2\sqrt{x}}\right)(a+\sqrt{x})}{(a-\sqrt{x})^2}\nonumber\\
&y'=\frac{\frac{a-\sqrt{x}+a+\sqrt{x}}{2\sqrt{x}}}{(a-\sqrt{x})^2}\nonumber\\
&y'=\frac{\frac{2a}{2\sqrt{x}}}{(a-\sqrt{x})^2}=\frac{2a}{2\sqrt{x}(\-\sqrt{x})^2}\nonumber\\
&y'=\frac{a}{x(a-\sqrt{x})^2}\nonumber
\end{align}
\end{ex}