%Exercicio81
%exercicio 172
\begin{ex}
\begin{align}
&\lim_{h\rightarrow 0} \frac{(x+h)^n-x^n}{h}=\nonumber\\
%resposta
&\text{como}\quad a^n-b^n=(a-b)(a^{n-1}+a^{n-2}.b+a^{n-3}.b^2+\dots+b^{n-1}), \text{temos:}\nonumber\\
&\lim_{h\rightarrow 0} \frac{(x+h-x)[(x+h)^{n-1}+(x+h)^{n-2}.x+(x+h)^{n-3}.x^2+\dots+x^{n-1}]}{h}=\nonumber\\
&\lim_{h\rightarrow 0} \frac{h[(x+h)^{n-1}+(x+h)^{n-2}.x+(x+h)^{n-3}.x^2+\dots+x^{n-1}]}{h}=\nonumber\\
&x^{n-1}+x^{n-2}.x+x^{n-3}.x^2+\dots+x^{n-1}=n.x^{n-1}\nonumber
\end{align}
\end{ex}