%Exercicio368
%exercicio 524 e 525
\begin{ex}
\begin{align}
&y=\tgh{x}\nonumber\\
%resposta
&y=\tgh{x} \Rightarrow y=\frac{e^{x}-e^{-x}}{e^{x}+e^{-x}}\nonumber\\
&y'=\frac{(e^{x}+e^{-x})(e^{x}-e^{-x})'-(e^{x}+e^{-x})'(e^{x}-e^{-x})}{(e^{x}+e^{-x})^2}\nonumber\\
&y'=\frac{(e^{x}+e^{-x})(e^{x}+e^{-x})-(e^{x}-e^{-x})(e^{x}-e^{-x})}{(e^{x}+e^{-x})^2}\nonumber\\
&y'=\frac{(e^{x}+e^{-x})^2-(e^{x}-e^{-x})^2}{(e^{x}+e^{-x})^2}\nonumber\\
&y'=\frac{(e^{x}+e^{-x}+e^{x}-e^{-x})(e^{x}+e^{-x}-e^{x}+e^{-x})}{(e^{x}+~e^{-x})^2}\nonumber\\
&y'=\frac{(2e^{x})(2e^{-x})}{(e^{x}+e^{-x})^2}=\frac{4}{(e^{x}+e^{-x})^2}=\frac{1}{\cosh^2{x}}\nonumber\\
&\text{De outra maneira:}\nonumber\\
&y=\tgh{x} \Rightarrow y=\frac{\senh{x}}{\cosh{x}}\nonumber\\
&y'=\frac{\cosh^2{x}-\senh^2{x}}{\cosh^2{x}}=\frac{1}{\cosh^2{x}}\nonumber
\end{align}
\end{ex}
