%Exercicio369
%exercicio 526 e 527
\begin{ex}
\begin{align}
&y=\cotgh{x}\nonumber\\
%resposta
&y=\cotgh{x} \Rightarrow y= \frac{e^{x}+e^{-x}}{e^{x}-e^{-x}}\nonumber\\
&y'=\frac{(e^{x}-e^{-x})(e^{x}+e^{-x})'-(e^{x}+e^{-x})(e^{x}-e^{-x})'}{(e^{x}-e^{-x})^2}\nonumber\\
&y'=\frac{(e^{x}-e^{-x})(e^{x}-e^{-x})-(e^{x}+e^{-x})(e^{x}+e^{-x})}{(e^{x}-e^{-x})^2}\nonumber\\
&y'=\frac{(e^{x}-e^{-x})^2-(e^{x}+e^{-x})^2}{(e^{x}-e^{-x})^2}\nonumber\\
&y'=\frac{(e^{x}-e^{-x}+e^{x}+e^{-x})(e^{x}-e^{-x}-e^{x}-e^{-x})}{(e^{x}-e^{-x})^2}\nonumber\\
&y'=\frac{(2e^{x})(-2e^{x})}{(e^{x}-e^{-x})^2}\nonumber\\
&y'=-\frac{1}{\senh^2{x}}\nonumber\\
&\text{De outra maneira:}\nonumber\\
&y=cotgh{x}=\frac{\cosh{x}}{\senh{x}}\nonumber\\
&y'=\frac{\senh^2{x}-\cosh^2{x}}{\senh^2{x}}\nonumber\\
&y'=-\frac{1}{\senh^2{x}}\nonumber
\end{align}
\end{ex}
