%Exercicio190
%exercicio 336
\begin{ex}
\begin{align}
&y=\frac{1+\sen{x}}{x\cos{x}}\nonumber\\
%resposta
&y'=\frac{(x\cos{x})(1+\sen{x})'-(x\cos{x})'(1+\sen{x})}{x^2\cos{x}^2}\nonumber\\
&y'=\frac{(x\cos{x})(\cos{x})-(1+\sen{x})[x(\cos{x})'+x'(\cos{x})]}{x^2\cos^2{x}}\nonumber\\
&y'=\frac{x\cos^2{x}-(1+\sen{x})[-x\sen{x}+\cos{x}]}{x^2\cos^2{x}}\nonumber\\
&y'=\frac{x\cos^2{x}+x\sen{x}^-\cos{x}+x\sen^2{x}-\sen{x}\cos{x}}{x^2\cos^2{x}}\nonumber\\
&y'=\frac{x+x\sen{x}-\cos{x}-\sen{x}\cos{x}}{x^2\cos^2{x}}\nonumber\\
&y'=\frac{x(1+\sen{x})-\cos{x}(1+\sen{x})}{x^2\cos^2{x}}\nonumber\\
&y'=\frac{(1+\sen{x})(x-\cos{x})}{x^2\cos^2{x}}\nonumber
\end{align}
\end{ex}