%Exercicio396
%exercicio 555
\begin{ex}
\begin{align}
&\lim_{x\rightarrow 0} \frac{e^{x}+\ln{(1-x)}-1}{\tg{x}-x}\nonumber\\
%resposta
&\lim_{x\rightarrow 0} \frac{e^{x}+\ln{(1-x)}-1}{\tg{x}-x}=\left[\frac{0}{0}\right]\nonumber\\
&\lim_{x\rightarrow 0} \frac{e^{x}-\frac{1}{(1-x)}}{\frac{1}{\cos^2{x}}-1}=\lim_{x\rightarrow 0} \frac{\cos^2{x}}{1-x}.\frac{e^{x}(1-x)-1}{1-\cos^2{x}}=\nonumber\\
&=1.\lim_{x\rightarrow 0} \frac{e^{x}(1-x)-1}{1-\cos^2{x}}=\nonumber\\
&=\lim_{x\rightarrow 0} \frac{e^{x}-e^{x}-xe^{x}}{2\sen{x}\cos{x}}=-\lim_{x\rightarrow 0} \frac{e^{x}}{2\cos{x}}.\lim_{x\rightarrow 0} \frac{x}{\sen{x}}=\nonumber\\
&=-\left(\frac{e^{x}}{2\cos{x}}\right).1=-\frac{1}{2}\nonumber
\end{align}
\end{ex}