%Exercicio284
%exercicio 440
\begin{ex}
\begin{align}
&y=3\sqrt[3]{\cos{2x}}(\cos^2{2x}-7)\nonumber\\
%resposta
&y'=\frac{-3(\cos^2{2x}-7)}{3\sqrt[3]{\cos^2{2x}}}2\sen{2x}+(-4\cos{2x}\sen{2x})3\sqrt[3]{\cos{x}}\nonumber\\
&y'=\frac{(\cos^2{2x}-7)2\sen{2x}+3\cos{2x}(-4\cos{2x}\sen{2x})}{\sqrt[3]{\cos^2{2x}}}\nonumber\\
&y'=\frac{14\sen{2x}-2\sen{2x}\cos^2{2x}-12\cos^2{2x}\sen{2x}}{\sqrt[3]{\cos^2{2x}}}\nonumber\\
&y'=\frac{14\sen{2x}(1-\cos^{2x})}{\sqrt[3]{\cos^2{2x}}}=\frac{14\sen^2{2x}}{\sqrt[3]{\cos^2{2x}}}\nonumber
\end{align}
\end{ex}