%Exercicio392
%exercicio 551 e 556
\begin{ex}
\begin{align}
&\lim_{x\rightarrow 0} \frac{x-\arcsen{x}}{x^3}\nonumber\\
%resposta
&\lim_{x\rightarrow 0} \frac{x-\arcsen{x}}{x^3}=\left[\frac{0}{0}\right]\nonumber\\
&\text{derivando duas vezes, temos:}\nonumber\\
&\lim_{x\rightarrow 0} \frac{-\frac{2x}{2\sqrt{1-x^2}}}{6x(1-x^2)-\frac{3x}{\sqrt{1-x^2}}}=\lim_{x\rightarrow 0} \frac{-1}{6-6x^2-3x^2}\nonumber\\
&\lim_{x\rightarrow 0} \frac{-1}{6-9x^2}=-\frac{1}{6}\nonumber\\
&\text{De outra maneira:}\nonumber\\
&\lim_{x\rightarrow 0} \frac{x-\arcsen{x}}{x^3}=\lim_{x\rightarrow 0} \frac{1-\frac{1}{\sqrt{1-x^2}}}{3x^2}\nonumber\\
&\lim_{x\rightarrow 0} \frac{\frac{\sqrt{1-x^2}-1}{\sqrt{1-x^2}}}{3x^2}=\lim_{x\rightarrow 0} \frac{\sqrt{1-x^2}-1}{3x^2(\sqrt{1-x^2})}=\nonumber\\
&\lim_{x\rightarrow 0} \frac{1}{\sqrt{1-x^2}}.\lim_{x\rightarrow 0} \frac{\sqrt{1-x^2}-1}{3x^2}=\nonumber\\
&1.\lim_{x\rightarrow 0} \frac{\frac{-2x}{2\sqrt{1-x^2}}}{6x}=1.\left(\frac{-1}{6}\right)=-\frac{1}{6}\nonumber
\end{align}
\end{ex} 