%Exercicio25
%exercicio 210
\begin{ex}
\begin{align}
&\lim_{x\rightarrow 0} \frac{\sqrt{x^2+1}-1}{\sqrt{x^2+16}-4}=\nonumber\\
%resposta
&\text{multiplicando e dividindo por}\nonumber\\
&(\sqrt{x^2+1}+1)(\sqrt{x^2+16}+4)\text{ , }\text{ temos: }\nonumber\\
&\lim_{x\rightarrow 0} \frac{(\sqrt{x^2+1}-1)[(\sqrt{x^2+1}+1)(\sqrt{x^2+16}+4)]}{(\sqrt{x^2+16}-4)[(\sqrt{x^2+1}+1)(\sqrt{x^2+16}+4)]}=\nonumber\\
&\lim_{x\rightarrow 0} \frac{(x^2-1+1)(\sqrt{x^2+16}+4)}{(x^2+16-16)(\sqrt{x^2+1}+1)}=\nonumber\\
&\lim_{x\rightarrow 0} \frac{\sqrt{x^2+16}+4}{\sqrt{x^2+1}+1}=\frac{16+4}{\sqrt{1}+1}=\frac{4+4}{2}=4\nonumber
\end{align}
\end{ex}