%Exercicio10
%exercicio 201
\begin{ex}
\begin{align}
&\lim_{x\rightarrow \infty} \sqrt{x^2-3x+7}-\sqrt{x^2+1}=\nonumber\\
%resposta
&\lim_{x\rightarrow \infty} \frac{(\sqrt{x^2-3x+7}-\sqrt{x^2+1})(\sqrt{x^2-3x+7}+\sqrt{x^2+1})}{\sqrt{x^2-3x+7}+\sqrt{x^2+1}}=\nonumber\\
&\lim_{x\rightarrow \infty} \frac{x^2-3x+7-x^2-1}{\sqrt{x^2-3x+7}+\sqrt{x^2+1}}=\lim_{x\rightarrow \infty} \frac{-3x+6}{\sqrt{x^2-3x+7}+\sqrt{x^2+1}}=\nonumber\\
&\lim_{x\rightarrow \infty} \frac{-\frac{3x}{x}+\frac{6}{x}}{\sqrt{\frac{x^2}{x^2}-\frac{3x}{x^2}+\frac{7}{x^2}}+\sqrt{\frac{x^2}{x^2}}+\frac{1}{x^2}}=\nonumber\\
&\lim_{x\rightarrow \infty}\frac{-3+\frac{6}{x}}{\sqrt{1-\frac{3}{x}+\frac{7}{x^2}}+\sqrt{1+\frac{1}{x^2}}}=\frac{-3}{\sqrt{1}+\sqrt{1}}=-\frac{3}{2}\nonumber
\end{align}
\end{ex}
