%Exercicio142
%exercicio 291
\begin{ex}
\begin{align}
&\lim_{h\rightarrow 0} \frac{f(x+h)-f(x)}{h}\quad\text{sendo}\quad f(x)=x^2-3x\nonumber\\
%resposta
&f(x+h)=(x+h)^2-3(x+h)=x^2+2xh+h^2-3x-3h\nonumber\\
&\lim_{h\rightarrow 0} \frac{f(x-h)-f(x)}{h}=\lim_{h\rightarrow 0} \frac{[(x+h)^2-3(x+h)]-(x^2-3x)}{h}\nonumber\\
&\lim_{h\rightarrow 0} \frac{x^2=2xh+h^2-3x-3h-x^2+3x}{h}=\nonumber\\
&\lim_{h\rightarrow 0} \frac{2xh+h^2-3h}{h}=\lim_{h\rightarrow 0} \frac{h(2x+h-3)}{h}=\nonumber\\
&\lim_{h\rightarrow 0} (2x+h+3)=2x-3\nonumber
\end{align}
\end{ex}