%Exercicio325
%exercicio 481
\begin{ex}
\begin{align}
&y=\ln{\frac{\sqrt{4+x^2}-2}{x}}\nonumber\\
%resposta
&y'=\frac{x}{\sqrt{4+x^2}-2}.\frac{\frac{x}{\sqrt{4+x^2}}.x-(\sqrt{4+x^2}-2)}{x^2}\nonumber\\
&y'=\frac{x^2-\sqrt{4+x^2}(\sqrt{4+x^2}-2)}{x\sqrt{4+x^2}(\sqrt{4+x^2}-2)}\nonumber\\
&y'=\frac{x}{4+x^2(\sqrt{4+x^2}-2)}-\frac{1}{x}=\frac{x(\sqrt{4+x^2}+2)}{x^2\sqrt{4+x^2}}-\frac{1}{x}\nonumber\\
&y'=\frac{\sqrt{4+x^2}+2-\sqrt{4+x^2}}{x\sqrt{4+x^2}}=\frac{2}{x\sqrt{4+x^2}}\nonumber
\end{align}
\end{ex}