%Exercicio244
%exercicio400
\begin{ex}
\begin{align}
&y=\left(\frac{1-\sqrt{1-x^2}}{x}\right)^4\nonumber\\
%resposta
&y'=4.\left(\frac{1-\sqrt{1-x^2}}{x}\right)^3.\frac{-x.\frac{-x}{\sqrt{1-x^2}}-1.(1-\sqrt{1-x^2})}{x^2}\nonumber\\
&y'=4\left(\frac{1-\sqrt{1-x^2}}{x}\right)^3.\frac{\frac{x^2}{\sqrt{1-x^2}}-1+\sqrt{1-x^2}}{x^2}\nonumber\\
&y'=4\left(\frac{1-\sqrt{1-x^2}}{x}\right)^3.\frac{x^2-\sqrt{1-x^2}+1-x^2}{x^2\sqrt{1-x^2}}\nonumber\\
&y'=\frac{4(1-\sqrt{1-x^2})^3}{x^3}.\frac{1-\sqrt{1-x^2}}{x^2\sqrt{1-x^2}}\nonumber\\
&y'=\frac{4(1-\sqrt{1-x^2})^4}{x^5\sqrt{1-x^2}}\nonumber
\end{align}
\end{ex}