%Exercicio323
%exercicio 479
\begin{ex}
\begin{align}
&y=3\left(\ln{\frac{1-\cos{2x}}{1+\cos{2x}}-\frac{2\cos{2x}}{\sen^2{2x}}}\right)+3\nonumber\\
%resposta
&y'=3\left[\frac{1+\cos{2x}}{1-\cos{2x}}.\frac{2\sen{2x}(1+\cos{2x})+2\sen{2x}(1-\cos{2x})}{(1+\cos{2x})^2}+\frac{4\sen{2x}\sen^2{2x}+4\sen{2x}\cos{2x}\cos{2x}}{\sen^4{2x}}\right]\nonumber\\
&y'=3\left[\frac{2\sen{2x}+2\sen{2x}\cos{2x}+2\sen{2x}-2\sen{2x}\cos{2x}}{1-\cos^2{2x}}+\frac{4\sen^3{2x}+8\sen{2x}\cos^2{2x}}{\sen^4{2x}}\right]\nonumber\\
&y'=3\left[\frac{4\sen{2x}}{\sen^2{2x}}+\frac{2\sen^2{2x}+8\cos^2{2x}}{\sen^3{2x}}\right]\nonumber\\
&y'=3\frac{4\sen^2{2x}+4\sen^2{2x}+8\cos^2{2x}}{\sen^3{2x}}=\frac{3.8}{\sen^3{2x}}\nonumber
\end{align}
\end{ex}
